theories/thunks/HThunks.v
@@ -6,21 +6,20 @@ From iris_time Require Import ThunksCode ThunksBase ThunksAPI ThunksFull.
 From iris_time Require Import Generations.
 Open Scope nat_scope.
 
-(* This file offers a theory of thunks indexed with integer generations.
+(* This file offers a theory of thunks indexed with integer heights.
    It is built on top of ThunksFull, which offers a more low-level theory
    of thunks indexed with masks. *)
 
-(* In both cases, this discipline aims to prevent the construction of
-   cyclic thunks. The main idea is that a thunk is allowed to force a
-   thunk of an earlier generation. It is *not* allowed to force a thunk
-   in the same generation or in a newer generation. A thunk is allowed
-   to *construct* a thunk in an arbitrary generation. *)
+(* In both cases, this discipline aims to prevent the construction of cyclic
+   thunks. The main idea is that a thunk is allowed to force a thunk at a
+   lower height. It is *not* allowed to force a thunk at the same height or
+   higher. A thunk is allowed to *construct* a thunk at an arbitrary height.  *)
 
 (* -------------------------------------------------------------------------- *)
 
 (* Prologue. *)
 
-Section GThunks.
+Section HThunks.
 
 Notation valO := (valO heap_lang).
 Context `{timeCreditHeapG Σ}.
@@ -31,11 +30,11 @@ Context `{na_invG Σ}.
 Notation iProp := (iProp Σ).
 Open Scope nat_scope.
 
-Definition generation := generation.
+Definition height := generation.
 
 Implicit Type p : na_inv_pool_name.
 Implicit Type t : loc.
-Implicit Type g : generation.
+Implicit Type h : height.
 Implicit Type n : nat.
 Implicit Type φ : val → iProp.
 
@@ -43,14 +42,14 @@ Implicit Type φ : val → iProp.
 
 (* The token associated with a pool [p] and bound [b]. *)
 
-Definition GToken p b :=
+Definition HToken p b :=
   na_own p (gens_below_bound b).
 
 (* This lemma allocates a new pool together with its token, which controls
-   all generations in this pool. *)
+   all heights in this pool. *)
 
 Lemma gtoken_alloc :
-  ⊢ |==> ∃ p, GToken p None.
+  ⊢ |==> ∃ p, HToken p None.
 Proof using.
     iApply na_alloc.
   Qed.
@@ -68,28 +67,27 @@ Proof using.
    file, we provide a simple discipline that removes most of this burden from
    the end user. *)
 
-(* The idea is simple: we index thunks with integer generations, and we allow
-   a thunk to force a thunk of an earlier generation. *)
+(* The idea is simple: we index thunks with integer heights, and we allow
+   a thunk to force a thunk at a lower height only. *)
 
 (* To do so, we use a thunk whose parameters [F] and [R] are instantiated in
    such a way that the tokens [ThunkToken p F] and [R] are disjoint. [F] is
-   instantiated with [↑(gen_ns g')], that is, control over the generation [g']
-   only. [R] is instantiated with [GToken p (Some g')], that is, control over
-   all generations below [g']. *)
+   instantiated with [↑(gen_ns h')], that is, control over the height [h']
+   only. [R] is instantiated with [HToken p (Some h')], that is, control over
+   all heights below [h']. *)
 
-(* An existential quantification over [g'], with the constraint [g' ≤ g],
-   ensures that [GThunk] is covariant in [g]. That is, it is safe to view
-   a thunk in an early generation as a thunk in a newer generation. *)
+(* An existential quantification over [h'], with the constraint [h' ≤ h],
+   ensures that [HThunk] is covariant in [h]. *)
 
 (* We could keep a parameterization in [R], so as to allow our thunks to have
    visible side effects (that is, side effects that require a token). We have
    not yet felt the need to do so; so, for the moment, a thunk is not allowed
    to have visible side effects other than forcing other thunks. *)
 
-Definition GThunk p g t n φ : iProp :=
-  ∃ g', ⌜ g' ≤ g ⌝ ∗
-  let F := ↑(gen_ns g') in
-  let R := GToken p (Some g') in
+Definition HThunk p h t n φ : iProp :=
+  ∃ h', ⌜ h' ≤ h ⌝ ∗
+  let F := ↑(gen_ns h') in
+  let R := HToken p (Some h') in
   Thunk p F t n R φ.
 
 (* -------------------------------------------------------------------------- *)
@@ -97,10 +95,10 @@ Definition GThunk p g t n φ : iProp :=
 (* Local tactics. *)
 
 Local Ltac deconstruct_thunk :=
-  iDestruct "Hthunk" as (g') "(% & Hthunk)".
+  iDestruct "Hthunk" as (h') "(% & Hthunk)".
 
-Local Ltac construct_thunk g' :=
-  iExists g'; iSplitR; [ eauto with lia |].
+Local Ltac construct_thunk h' :=
+  iExists h'; iSplitR; [ eauto with lia |].
 
 Local Ltac construct_texan_triple ipat :=
   iIntros "#?"; (* introduce TC_invariant *)
@@ -110,113 +108,113 @@ Local Ltac construct_texan_triple ipat :=
 
 (* -------------------------------------------------------------------------- *)
 
-(* [GThunk] is persistent. *)
+(* [HThunk] is persistent. *)
 
-Global Instance gthunk_persistent p g t n φ :
-  Persistent (GThunk p g t n φ).
+Global Instance hthunk_persistent p h t n φ :
+  Persistent (HThunk p h t n φ).
 Proof using.
   exact _.
 Qed.
 
 (* -------------------------------------------------------------------------- *)
 
-(* The creation rule passes the token [GToken p (Some g)] to the suspended
-   computation [f]. Thus, the newly created thunk, which belongs in the
-   generation [g], can force thunks in generations less than [g]. *)
+(* The creation rule passes the token [HToken p (Some h)] to the suspended
+   computation [f]. Thus, the newly created thunk, which lies at height [h],
+   can force thunks at heights less than [h]. *)
 
 (* There is no restriction regarding the thunks that this new thunk may
    construct. Indeed, the postcondition [φ] is arbitrary. *)
 
-Lemma gthunk_create p g n φ f :
-  let token := GToken p (Some g) in
+Lemma hthunk_create p h n φ f :
+  let token := HToken p (Some h) in
   TC_invariant -∗
   {{{ TC 3 ∗ isAction f n token φ }}}
     « create f »
-  {{{ t, RET «#t» ; GThunk p g t n φ }}}.
+  {{{ t, RET «#t» ; HThunk p h t n φ }}}.
 Proof.
   construct_texan_triple "H".
   wp_apply (thunk_create with "[$] H"); [ done |].
   iIntros (t) "Hthunk".
-  iApply "Post". construct_thunk g. done.
+  iApply "Post". construct_thunk h. done.
 Qed.
 
 (* -------------------------------------------------------------------------- *)
 
 (* The consequence rule is standard. *)
 
-Lemma gthunk_consequence p g t n1 n2 φ ψ E :
+Lemma hthunk_consequence p h t n1 n2 φ ψ E :
   (∀ v, TC n2 -∗ □ φ v ={⊤}=∗ □ ψ v) -∗
-  GThunk p g t  n1       φ  ={E}=∗
-  GThunk p g t (n1 + n2) ψ.
+  HThunk p h t  n1       φ  ={E}=∗
+  HThunk p h t (n1 + n2) ψ.
 Proof.
   iIntros "Hupdate Hthunk".
   deconstruct_thunk.
   iMod (thunk_consequence with "Hthunk [Hupdate]").
-  { (* The token [GToken p (Some g')] is not passed to the update,
-       because it would be essentially useless, as [g'] is unknown. *)
+  { (* The token [HToken p (Some h')] is not passed to the update,
+       because it would be essentially useless, as [h'] is unknown. *)
     iIntros (v) "$ Htc Hv".
     iApply ("Hupdate" with "Htc").
     iAssumption. }
-  iModIntro. construct_thunk g'. done.
+  iModIntro. construct_thunk h'. done.
 Qed.
 
 (* -------------------------------------------------------------------------- *)
 
-(* [GThunk] is covariant in the parameter [g]. That is, it is safe to view a
-   thunk in an early generation as a thunk in a newer generation. This makes
-   this thunk more difficult to force, as a stronger token is required. *)
+(* [HThunk] is covariant in the parameter [h]. That is, it is safe to view a
+   thunk at a low height as a thunk at a greater height. This makes this thunk
+   more difficult to force, as a stronger token is required. *)
 
-Lemma gthunk_covariant_in_g p g1 g2 t n φ :
-  g1 ≤ g2 →
-  GThunk p g1 t n φ -∗
-  GThunk p g2 t n φ.
+Lemma hthunk_covariant_in_h p h1 h2 t n φ :
+  h1 ≤ h2 →
+  HThunk p h1 t n φ -∗
+  HThunk p h2 t n φ.
 Proof.
   iIntros (?) "Hthunk".
   deconstruct_thunk.
-  construct_thunk g'.
+  construct_thunk h'.
   done.
 Qed.
 
 (* -------------------------------------------------------------------------- *)
 
-(* [GThunk] is covariant in the parameter [n]. That is, it is safe to view a
+(* [HThunk] is covariant in the parameter [n]. That is, it is safe to view a
    thunk with a small debt as a thunk with a greater debt. *)
 
-Lemma gthunk_increase_debt p g t n1 n2 φ :
+Lemma hthunk_increase_debt p h t n1 n2 φ :
   n1 ≤ n2 →
-  GThunk p g t n1 φ -∗
-  GThunk p g t n2 φ.
+  HThunk p h t n1 φ -∗
+  HThunk p h t n2 φ.
 Proof using.
   iIntros (?) "Hthunk".
   deconstruct_thunk.
-  construct_thunk g'.
+  construct_thunk h'.
   by iApply thunk_increase_debt.
 Qed.
 
 (* -------------------------------------------------------------------------- *)
 
-(* Forcing a thunk in a generation [g] that lies below the bound [b] requires
-   the token [GToken p b]. *)
+(* Forcing a thunk at height [h] that lies below the bound [b] requires the
+   token [HToken p b]. *)
 
-(* To solve the proof obligation [lies_below g b], use [eauto with thunks].   *)
+(* To solve the proof obligation [lies_below h b], use [eauto with thunks].   *)
 
 (* The thunk must have zero debit. If it has more than zero debit, then [pay]
-   and [force] must be composed; see [gthunk_pay_force] below. *)
+   and [force] must be composed; see [hthunk_pay_force] below. *)
 
-Lemma gthunk_force p g b t φ :
-  lies_below g b →
-  let token := GToken p b in
+Lemma hthunk_force p h b t φ :
+  lies_below h b →
+  let token := HToken p b in
   TC_invariant -∗
-  {{{ TC 11 ∗ GThunk p g t 0 φ ∗ token }}}
+  {{{ TC 11 ∗ HThunk p h t 0 φ ∗ token }}}
     « force #t »
   {{{ v, RET «v» ; □ φ v ∗ ThunkVal t v ∗ token }}}.
 Proof using.
-  intros Hg.
+  intros Hh.
   construct_texan_triple "(Htc & Hthunk & Htoken)".
   deconstruct_thunk.
-  assert (Hg': lies_below g' b) by eauto using leq_lies_below.
-  rewrite /GToken.
-  rewrite (carve_out_gens_below_gen _ _ Hg').
+  assert (Hh': lies_below h' b) by eauto using leq_lies_below.
+  rewrite /HToken.
+  rewrite (carve_out_gens_below_gen _ _ Hh').
   iDestruct (na_own_union with "Htoken") as "[Htoken1 Htoken2]".
   { set_solver. }
   (* Both tokens are required here. *)
@@ -234,20 +232,20 @@ Qed.
 
 (* Forcing a thunk that has already been forced. See ThunksAPI for comments. *)
 
-Lemma gthunk_force_forced p g t n φ b v :
-  lies_below g b →
-  let token := GToken p b in
+Lemma hthunk_force_forced p h t n φ b v :
+  lies_below h b →
+  let token := HToken p b in
   TC_invariant -∗
-  {{{ TC 11 ∗ GThunk p g t n φ ∗ ThunkVal t v ∗ token }}}
+  {{{ TC 11 ∗ HThunk p h t n φ ∗ ThunkVal t v ∗ token }}}
     « force #t »
   {{{ RET «v» ; token }}}.
 Proof using.
-  intros Hg.
+  intros Hh.
   construct_texan_triple "(Htc & Hthunk & Hval & Htoken)".
   deconstruct_thunk.
-  assert (Hg': lies_below g' b) by eauto using leq_lies_below.
-  rewrite /GToken.
-  rewrite (carve_out_gens_below_gen _ _ Hg').
+  assert (Hh': lies_below h' b) by eauto using leq_lies_below.
+  rewrite /HToken.
+  rewrite (carve_out_gens_below_gen _ _ Hh').
   iDestruct (na_own_union with "Htoken") as "[Htoken1 Htoken2]".
   { set_solver. }
   (* Only one token is required here. *)
@@ -265,38 +263,38 @@ Qed.
 
 (* Paying. *)
 
-Lemma gthunk_pay k E p g t n φ :
+Lemma hthunk_pay k E p h t n φ :
   ↑ThunkPayment ⊆ E →
-  GThunk p g t n φ -∗ TC k
+  HThunk p h t n φ -∗ TC k
     ={E}=∗
-  GThunk p g t (n-k) φ.
+  HThunk p h t (n-k) φ.
 Proof using.
   iIntros (?) "Hthunk Htc".
   deconstruct_thunk.
   iMod (thunk_pay with "Hthunk Htc"); [ done |].
-  iModIntro. construct_thunk g'. done.
+  iModIntro. construct_thunk h'. done.
 Qed.
 
 (* -------------------------------------------------------------------------- *)
 
 (* The composition of [pay] and [force]. *)
 
-Lemma gthunk_pay_force p g b t d φ :
-  lies_below g b →
-  let token := GToken p b in
+Lemma hthunk_pay_force p h b t d φ :
+  lies_below h b →
+  let token := HToken p b in
   TC_invariant -∗
-  {{{ TC (11 + d) ∗ GThunk p g t d φ ∗ token }}}
+  {{{ TC (11 + d) ∗ HThunk p h t d φ ∗ token }}}
     « force #t »
   {{{ v, RET «v» ; □ φ v ∗ ThunkVal t v ∗ token }}}.
 Proof.
-  intros Hg.
+  intros Hh.
   iIntros "#HtickInv" (Φ) "!# ((Htc1 & Htc2) & #Hthunk & Htoken) Post".
-  iMod (gthunk_pay with "Hthunk Htc2") as "#Hthunk'"; [ done |].
+  iMod (hthunk_pay with "Hthunk Htc2") as "#Hthunk'"; [ done |].
   iClear "Hthunk". iRename "Hthunk'" into "Hthunk".
-  wp_apply (gthunk_force with "[$] [$Htc1 Hthunk $Htoken]").
+  wp_apply (hthunk_force with "[$] [$Htc1 Hthunk $Htoken]").
   { done. }
   { rewrite Nat.sub_diag. iFrame "Hthunk". }
   eauto.
 Qed.
 
-End GThunks.
+End HThunks.
